Clean/Gadgets/BLAKE3/ApplyRounds.lean
@@ -475,9 +475,7 @@ lemma initial_state_and_messages_are_normalized
   -- Helper to prove normalization of chaining value elements
   have h_chaining_value_normalized (i : ℕ) (h_i : i < 8) : (eval env input_var_chaining_value[i]).Normalized := by
     simp_all only [circuit_norm, eval_vector_eq_get]
-    convert h_normalized.1 i
-    norm_num
-    omega
+    convert h_normalized.1 ⟨ i, h_i ⟩
 
   -- Show the state is normalized
   have h_state_normalized : (eval env state_vec).Normalized := by
@@ -490,7 +488,7 @@ lemma initial_state_and_messages_are_normalized
     -- Next 4 are IV constants
     case «8» | «9» | «10» | «11» => state_vec_norm_simp_simple
     -- Last 4 are counter_low, counter_high, block_len, flags
-    case «12» |«13» | «14» | «15» => state_vec_norm_simp_simple; simp_all [Assumptions, h_input]
+    case «12» |«13» | «14» | «15» => state_vec_norm_simp_simple; simp_all
 
   constructor
   · apply h_state_normalized
